got rid of the final remaining admits
now that we have agreed on the constants for fold

common/array.v
@@ -4,41 +4,6 @@ Require Import Braun.common.log.
 Require Import Braun.common.util Braun.common.le_util.
 Require Import Arith Arith.Even Arith.Div2 List.
 
-Fixpoint man_time n : nat :=
-  match n with
-    | 0 => 0
-    | S n' => man_time n' + (cl_log n)
-  end.
-
-Example man_time_ex :
-  map man_time (1 :: 2 :: 3 :: 4 ::  5 ::  6 ::  7 ::  8 ::  9 :: 10 :: nil)
-             = (1 :: 3 :: 5 :: 8 :: 11 :: 14 :: 17 :: 21 :: 25 :: 29 :: nil).
-Proof.
-  auto.
-Qed.
-
-Lemma man_time_nlogn :
-  forall n,
-    man_time n <= n * cl_log n.
-Proof.
-  induction n as [|n].
-
-  simpl; omega.
-
-  replace (S n * cl_log (S n)) with (n * cl_log (S n) + cl_log (S n));
-    [|unfold mult; fold mult; omega].
-  unfold man_time; fold man_time.
-  apply le_plus_left.
-  apply (le_trans (man_time n)
-                  (n * cl_log n)
-                  (n * cl_log (S n))).
-  assumption.
-  
-  apply le_mult_right.
-  apply cl_log_monotone.
-Qed.
-Hint Resolve man_time_nlogn.
-
 (* this is http://oeis.org/A001855 *)
 Program Fixpoint mat_time n {measure n} :=
   match n with
@@ -88,15 +53,6 @@ Proof.
   replace (div2 (S (S n))) with (S (div2 n));[|unfold div2;reflexivity].
 
   omega.
-Qed.
-
-Lemma rt_naive_same_as_mat_time :
-  forall n, mat_time n = man_time n.
-Proof.
-  induction n.
-  auto.
-  
-  simpl; rewrite <- IHn; apply mat_time_Sn_cl_log; auto.
 Qed.
 
 Lemma braun_implies_mat_time:
