logical/make_array_naive.v
@@ -72,6 +72,34 @@ Proof.
 Qed.
 Hint Resolve MakeArrayNaiveR_correct.
 
+Fixpoint man_time n : nat :=
+  match n with
+    | 0 => 0
+    | S n' => man_time n' + (cl_log n)
+  end.
+
+Lemma man_time_nlogn :
+  forall n,
+    man_time n <= n * cl_log n.
+Proof.
+  induction n as [|n].
+
+  simpl; omega.
+
+  replace (S n * cl_log (S n)) with (n * cl_log (S n) + cl_log (S n));
+    [|unfold mult; fold mult; omega].
+  unfold man_time; fold man_time.
+  apply le_plus_left.
+  apply (le_trans (man_time n)
+                  (n * cl_log n)
+                  (n * cl_log (S n))).
+  assumption.
+  
+  apply le_mult_right.
+  apply cl_log_monotone.
+Qed.
+Hint Resolve man_time_nlogn.
+
 Theorem MakeArrayNaiveR_time :
   forall A xs (bt:@bin_tree A) t,
     MakeArrayNaiveR xs bt t ->
