tmonad/make_array_naive_fold.v
@@ -6,7 +6,7 @@ Require Import Braun.logical.sequence.
 
 Require Import Braun.common.braun.
 Require Import Braun.common.array.
-Require Import Braun.common.util.
+Require Import Braun.common.util Braun.common.big_oh.
 Require Import Braun.common.log Braun.common.le_util.
 Require Import Arith Arith.Even Arith.Div2 Omega.
 
@@ -14,36 +14,127 @@ Require Import Arith Arith.Even Arith.Div2 Omega.
 Section make_array_naive.
   Variable A : Set.
   
-  Definition man_correct (b : @bin_tree A) (xs : list A) (c : nat) : Prop :=
+  Fixpoint man_time n : nat :=
+    match n with
+      | 0 => 4
+      | S n' => man_time n' + insert_time n' + 14
+    end.
+
+  Definition make_array_naive_result (b : @bin_tree A) (xs : list A) (c : nat) : Prop :=
     let n := length xs in
     Braun b n
     /\ c = man_time n
     /\ SequenceR b xs.
-
+  
+  (* technically, we should count 4 more for the call to foldr,
+     but that means that we cannot use make_array_naive_result
+     as the loop invariant argument to foldr so we just skip it *)
   Program Definition make_array_naive l : 
     {! b !:! @bin_tree A !<! c !>!
-       man_correct b l c !} :=
-    foldr man_correct
-          (fun x y => x <- insert x y; <== x)
+       make_array_naive_result b l c !} :=
+    foldr make_array_naive_result
+          (fun x y => x <- insert x y; +=4; <== x)
           bt_mt
           l.
+
   Next Obligation.
-    clear xm H1.
-    rename H into IR.
-    rename H0 into MC.
+  Proof.
+    clear xm H2.
+    rename H0 into IR.
+    rename H1 into MC.
 
     unfold insert_result in IR.
     destruct MC as [BRy [ACCCeq SR]].
-    unfold man_correct.
+    unfold make_array_naive_result.
     remember (IR (length xs) BRy) as IRlxs.
     destruct IRlxs as [BRx0 [SRimpl EQxn]].
     simpl.
     repeat split;auto.
-    admit. (* running time; pending running time decision of fold *)
+    omega.
   Qed.
+
   Next Obligation.
-    unfold man_correct.
+  Proof.
+    unfold make_array_naive_result.
     repeat split; auto.
-    admit. (* running time; pending running time decision of fold *)
   Qed.
+
+  Lemma man_time_helper:
+    forall n,
+      man_time n <= n * insert_time n + (n * 14) + 4.
+    Proof.
+      intros n.
+      induction n as [|n].
+      simpl; omega.
+      unfold man_time; fold man_time.
+      apply (le_trans (man_time n + insert_time n + 14)
+                      ((n * insert_time n + n * 14 + 4)  + insert_time n + 14)
+                      (S n * insert_time (S n) + S n * 14 + 4)); try omega.
+      clear IHn.
+      replace (S n * insert_time (S n)) with (n * insert_time (S n) + insert_time (S n)).
+
+      assert (insert_time n <= insert_time (S n)) as ITLT.
+      unfold insert_time.
+      apply le_plus_left.
+      apply le_mult_right.
+      apply fl_log_monotone.
+
+      assert (n * insert_time n <= n * insert_time (S n)) as NITLT.
+      apply le_mult_right.
+      assumption.
+
+      omega.
+
+      assert (S n = n+1) as SN;try omega.
+      rewrite SN at 3; clear SN.
+      rewrite mult_plus_distr_r.
+      omega.
+    Qed.
+
+  Theorem man_time_nlogn : big_oh man_time (fun n => n * fl_log n).
+  Proof.
+    apply (big_oh_trans man_time
+                        (fun n => n * fl_log n + n + 10)
+                        (fun n => n * fl_log n)).
+    exists 0.
+    exists 20.
+    intros n H; clear H.
+    apply (le_trans (man_time n)
+                    (n * insert_time n + (n * 14) + 4)
+                    (20*(n * fl_log n + n + 10))).
+    apply man_time_helper.
+    unfold insert_time.
+    repeat (rewrite mult_plus_distr_l).
+    repeat (rewrite mult_assoc).
+    replace (n * 9 * fl_log n) with (9 * n * fl_log n).
+    replace (n * 6) with (6 * n); try (apply mult_comm).
+    replace (n * 14) with (14 * n); try (apply mult_comm).
+    replace (9 * n * fl_log n + 6 * n + 14 * n + 4)
+    with (9 * n * fl_log n + 20 * n + 4); try omega.
+
+    assert (9 * n * fl_log n <=  20 * n * fl_log n); try omega.
+    apply le_mult_left.
+    apply le_mult_left.
+    omega.
+
+    rewrite (mult_comm 9).
+    reflexivity.
+
+    apply (big_oh_trans (fun n => n * fl_log n + n + 10)
+                        (fun n => n * fl_log n + n)
+                        (fun n => n * fl_log n)).
+    exists 1.
+    exists 11.
+    intros n L.
+    destruct n; intuition.
+    clear L.
+    rewrite mult_plus_distr_l.
+
+    assert ((S n * fl_log (S n)) <= 11 * (S n * fl_log (S n))); try omega.
+    remember (mult_O_le (S n * fl_log (S n)) 11) as FACT.
+    inversion FACT; intuition.
+
+    apply big_oh_nlogn_plus_n__nlogn.
+  Qed.
+
 End make_array_naive.
